arrays/spec/new.v
@@ -1,0 +1,164 @@
+From iris.algebra Require Import auth frac_auth gset.
+From iris.heap_lang Require Import proofmode.
+
+From SkipList.lib Require Import lock misc node_rep node_lt key_equiv.
+From SkipList.arrays Require Import code.
+From SkipList.arrays.inv Require Import list_equiv lazy_inv skip_inv.
+
+
+Module NewSpec (Params: SKIP_LIST_PARAMS).
+  Import Params.
+  Module Invariant := SkipListInv Params.
+  Export Invariant.
+
+  Section Proofs.
+    Context `{!heapGS Σ, !gset_list_unionGS Σ, !lockG Σ}.
+
+    Theorem array_inv (lvl: nat) (head: node_rep) (t: loc)
+      (bot: bot_gname) (subs: list sub_gname) (γ: gname):
+      skip_list_equiv lvl head ∅ 1 bot subs
+      ∗
+      is_lock γ (node_lock head) (node_inv (node_next head))
+      ∗
+      t ↦{#1 / exp2 (lvl + 1)} rep_to_node tail
+      ∗
+      (node_next head +ₗ lvl +ₗ 1) ↦∗{#1 / 2} replicate (MAX_HEIGHT - lvl) #t 
+      ∗
+      ⌜ 0 ≤ lvl ≤ MAX_HEIGHT ⌝ 
+      ∗
+      ⌜ node_key head = INT_MIN ⌝ 
+      ={⊤}=∗
+        ∃ (subs: list sub_gname), 
+          skip_list_equiv MAX_HEIGHT head ∅ 1 bot subs.
+    Proof.
+      remember (MAX_HEIGHT - lvl) as diff eqn:Hdiff.
+      iRevert (lvl subs Hdiff).
+      iInduction diff as [|d] "IHdiff";
+        iIntros (lvl subs Hdiff) "(Hlist & #Hlock & Ht & Hnext & %Hmax & %Hmin)".
+
+      + assert (lvl = MAX_HEIGHT) as -> by lia.
+        iModIntro. iExists subs. iFrame.
+      + destruct subs as [| top_sub bot_subs]; first by iExFalso.
+
+        rewrite replicate_S array_cons.
+        iDestruct "Hnext" as "(Hnext' & Hnext)".
+        iDestruct "Ht" as "(Ht & Ht')".
+
+        iMod (own_alloc (● (∅ : gset node_rep) ⋅ ◯ (∅: gset node_rep)))
+          as (γauth) "[Hown_auth _]"; 
+          first by apply auth_both_valid.
+        iMod (own_alloc (GSet node_key_range))
+          as (γtoks) "Hown_toks"; first done.
+        assert (node_key_range = node_key_range ∖ ∅) as -> by set_solver.
+
+        set (sub := mk_sub_gname γauth γtoks).
+        iMod (inv_alloc (levelN (lvl + 1)) ⊤ (lazy_list_inv (lvl + 1) head sub None (from_top_list top_sub)) 
+          with "[Hnext' Ht' Hown_auth Hown_toks]") as "Hinv".
+        {
+          iNext; iExists ∅, ∅, nil. iFrame.
+          iSplit; first done. iSplit.
+          {
+            assert (node_lt head tail); last (simpl; auto).
+            rewrite /node_key in Hmin.
+            rewrite /node_lt /node_key Hmin /=; apply HMIN_MAX.
+          }
+          iSplit; first rewrite /key_equiv //.
+          iExists γ, t. 
+          rewrite loc_add_assoc.
+          assert (lvl + 1 + 1 = S (lvl + 1)) as -> by lia.
+          assert ((lvl + 1)%Z = lvl + 1) as -> by lia.
+          rewrite Qp_div_div comm_L //=.
+          iFrame "# ∗".
+        }
+
+        iApply ("IHdiff" $! (lvl + 1) (sub :: top_sub :: bot_subs) with "[%]").
+        { lia. }
+
+        iSplitL "Hinv Hlist".
+        {
+          rewrite /skip_list_equiv.
+          assert (lvl + 1 - 1 = lvl) as -> by lia.
+          iFrame "# ∗". iPureIntro; lia.
+        }
+
+        rewrite Qp_div_div comm_L //=.
+        assert (lvl + 1 + 1 = S (lvl + 1)) as -> by lia.
+        assert ((lvl + 1)%Z = lvl + 1) as <- by lia.
+        rewrite -loc_add_assoc.
+        iFrame "# ∗". iPureIntro.
+        by split; first lia.
+    Qed.
+
+    Theorem new_spec : 
+      {{{ True }}}
+        new #()
+      {{{ v bot subs, RET v; is_skip_list v ∅ 1 bot subs }}}.
+    Proof.
+      iIntros (Φ) "_ HΦ".
+
+      wp_lam. wp_alloc t as "Ht". wp_let.
+      wp_alloc next as "Hnext"; first lia. wp_let.
+      assert (Z.to_nat (MAX_HEIGHT + 1) = S MAX_HEIGHT) as -> by lia.
+      iDestruct "Hnext" as "(Hnext' & Hnext)".
+
+      wp_apply (newlock_spec (node_inv next) with "[Hnext']").
+      { iExists (replicate (S MAX_HEIGHT) #t); iFrame. }
+      iIntros (l) "#Hlock". iDestruct "Hlock" as (γ) "Hlock".
+
+      rewrite replicate_S array_cons.
+      iDestruct "Hnext" as "(Hnext' & Hnext)".
+      iDestruct "Ht" as "(Ht & Ht')".
+
+      wp_pures.
+      rewrite (fold_rep_to_node (INT_MIN, next, None, l)).
+      set (head := (INT_MIN, next, None, l)).
+
+      iMod (own_alloc (● (∅ : gset node_rep) ⋅ ◯ (∅: gset node_rep)))
+        as (γauth) "[Hown_auth Hown_auth_frag]"; 
+        first by apply auth_both_valid.
+      iMod (own_alloc (GSet node_key_range))
+        as (γtoks) "Hown_toks"; 
+        first done.
+      iMod (own_alloc (●F (∅ : gset Z) ⋅ ◯F (∅: gset Z)))
+        as (γfrac) "[Hown_frac Hown_frac_frag]"; 
+        first by apply auth_both_valid.
+      assert (node_key_range = node_key_range ∖ ∅) as -> by set_solver.
+
+      set (sub := mk_sub_gname γauth γtoks).
+      set (bot := mk_bot_gname γfrac).
+      iMod (inv_alloc (levelN 0) ⊤ (lazy_list_inv 0 head sub (Some bot) from_bot_list) 
+        with "[Hnext' Ht' Hown_auth Hown_toks Hown_frac]") as "Hinv".
+      {
+        iNext; iExists ∅, ∅, nil. iFrame.
+        iSplit; first done. iSplit.
+        {
+          assert (node_lt head tail); last (simpl; auto).
+          rewrite /node_lt/node_key//=; apply HMIN_MAX.
+        }
+        iSplit; first rewrite /key_equiv //.
+        iExists γ, t.
+        rewrite loc_add_0 /node_next /= Qp_mul_1_r.
+        iFrame "# ∗".
+      }
+
+      iAssert (skip_list_equiv 0 head ∅ 1 bot [sub]) 
+        with "[Hinv Hown_frac_frag]" as "Hskip".
+      { by iFrame. }
+
+      iPoseProof (array_inv 0 head t bot [sub] γ with "[Hskip Hlock Ht Hnext]") as "Hskip".
+      {
+        rewrite loc_add_assoc /node_next /= Qp_mul_1_r. 
+        assert (0%nat + 1 = 1)%Z as -> by lia.
+        assert (MAX_HEIGHT - 0 = MAX_HEIGHT) as -> by lia.
+        iFrame "# ∗". iPureIntro.
+        by split; first lia.
+      }
+      iMod "Hskip" as (subs) "Hskip".
+
+      wp_alloc h as "Hh".
+      iModIntro; iApply ("HΦ" $! _ bot subs).
+      iExists h, head. by iFrame.
+    Qed.
+
+  End Proofs.
+End NewSpec.
